src/lib/crypto/DY.Lib.Crypto.Signature.Split.fst
@@ -5,44 +5,43 @@ open DY.Core
 open DY.Lib.Crypto.SplitPredicate
 
 let split_sign_predicate_params {|crypto_usages|}: split_crypto_predicate_parameters = {
-  key_t = vk:bytes{SigKey? (get_signkey_usage vk)};
+  key_usage_t = sk_usage:usage{SigKey? sk_usage};
   data_t = bytes;
-  get_usage = (fun pk ->
-    let SigKey tag _ = get_signkey_usage pk in
+  get_usage = (fun vk_usg ->
+    let SigKey tag _ = vk_usg in
     tag
   );
 
   local_pred_t = sign_crypto_predicate;
-  global_pred_t = tr:trace -> vk:bytes{SigKey? (get_signkey_usage vk)} -> msg:bytes -> prop;
+  global_pred_t = tr:trace -> sk_usage:usage{SigKey? sk_usage} -> msg:bytes -> prop;
 
-  apply_local_pred = (fun pred (tr, vk, msg) ->
-    pred.pred tr vk msg
+  apply_local_pred = (fun pred (tr, sk_usage, msg) ->
+    pred.pred tr sk_usage msg
   );
-  apply_global_pred = (fun pred (tr, vk, msg) ->
-    pred tr vk msg
+  apply_global_pred = (fun pred (tr, sk_usage, msg) ->
+    pred tr sk_usage msg
   );
-  mk_global_pred = (fun pred tr vk msg ->
-    pred (tr, vk, msg)
+  mk_global_pred = (fun pred tr sk_usage msg ->
+    pred (tr, sk_usage, msg)
   );
 
-  key_and_data_well_formed = (fun tr vk msg ->
-    bytes_well_formed tr vk /\
+  data_well_formed = (fun tr msg ->
     bytes_well_formed tr msg
   );
 
   apply_mk_global_pred = (fun bare x -> ());
-  apply_local_pred_later = (fun lpred tr1 tr2 vk msg ->
-    lpred.pred_later tr1 tr2 vk msg
+  apply_local_pred_later = (fun lpred tr1 tr2 sk_usage msg ->
+    lpred.pred_later tr1 tr2 sk_usage msg
   );
 }
 
 val has_sign_predicate: {|crypto_invariants|} -> (string & sign_crypto_predicate) -> prop
 let has_sign_predicate #cinvs (tag, local_pred) =
-  forall (tr:trace) (vk:bytes) (msg:bytes).
-    {:pattern sign_pred.pred tr vk msg}
-    match get_signkey_usage vk with
+  forall (tr:trace) (sk_usage:usage) (msg:bytes).
+    {:pattern sign_pred.pred tr sk_usage msg}
+    match sk_usage with
     | SigKey sign_tag _ ->
-        sign_tag = tag ==> sign_pred.pred tr vk msg == local_pred.pred tr vk msg
+        sign_tag = tag ==> sign_pred.pred tr sk_usage msg == local_pred.pred tr sk_usage msg
     | _ -> True
 
 val intro_has_sign_predicate:
@@ -52,15 +51,15 @@ val intro_has_sign_predicate:
   (ensures has_sign_predicate tagged_local_pred)
 let intro_has_sign_predicate #cinvs (tag, local_pred) =
   introduce
-    forall tr vk msg.
-      match get_signkey_usage vk with
+    forall tr sk_usage msg.
+      match sk_usage with
       | SigKey sign_tag _ ->
-          sign_tag = tag ==> sign_pred.pred tr vk msg == local_pred.pred tr vk msg
+          sign_tag = tag ==> sign_pred.pred tr sk_usage msg == local_pred.pred tr sk_usage msg
       | _ -> True
   with (
-    match get_signkey_usage vk with
+    match sk_usage with
     | SigKey sign_tag _ ->
-      has_local_crypto_predicate_elim (split_sign_predicate_params) sign_pred.pred tag local_pred tr vk msg
+      has_local_crypto_predicate_elim (split_sign_predicate_params) sign_pred.pred tag local_pred tr sk_usage msg
     | _ -> ()
   )
 
